Several simplifications in proofs

formal-proofs/theories/lib/thread_queue/thread_queue.v
@@ -16,7 +16,7 @@ Definition cancel_cell: val :=
   λ: "cell'",
   let: "cell" := cell_ref_loc "cell'" in
   if: getAndSet "cell" CANCELLEDV = RESUMEDV
-  then segment_cancel_cell (Fst "cell")
+  then segment_cancel_single_cell (Fst "cell")
   else #().
 
 Definition move_ptr_forward : val :=
@@ -61,6 +61,7 @@ Definition resume: val :=
 End impl.
 
 From iris.heap_lang Require Import proofmode.
+From iris.algebra Require Import auth.
 
 Section proof.
 
@@ -74,26 +75,39 @@ Let segment_size := p_segment_size ap.
 
 Context `{iArrayG Σ}.
 
-Theorem move_ptr_forward_spec γ (v: loc) id ℓ:
-  segment_location γ id ℓ -∗
+Class iArrayPtrG Σ := IArrayPtrG { iarrayptr_inG :> inG Σ (authUR mnatUR) }.
+Definition iArrayPtrΣ : gFunctors := #[GFunctor (authUR mnatUR)].
+Instance subG_iArrayPtrΣ {Σ} : subG iArrayPtrΣ Σ -> iArrayPtrG Σ.
+Proof. solve_inG. Qed.
+
+Context `{iArrayPtrG Σ}.
+
+Definition ptr_points_to_segment γa γ ℓ id :=
+  (∃ (ℓ': loc), ℓ ↦ #ℓ' ∗ segment_location γa id ℓ' ∗ own γ (● (id: mnatUR)))%I.
+
+Theorem move_ptr_forward_spec γa γ (v: loc) id ℓ:
+  segment_location γa id ℓ -∗
   ([∗ list] j ∈ seq 0 (id * Pos.to_nat segment_size), cell_is_processed j) -∗
-  <<< ∀ (id': nat) (ℓ': loc), ▷ is_infinite_array ap γ ∗ v ↦ #ℓ' ∗
-                                         segment_location γ id' ℓ' >>>
+  <<< ∀ (id': nat), ▷ is_infinite_array ap γa ∗ ptr_points_to_segment γa γ v id' >>>
     move_ptr_forward #v #ℓ @ ⊤
-  <<< ▷ is_infinite_array ap γ ∗ (⌜id > id'⌝ ∗ v ↦ #ℓ ∨ ⌜id <= id'⌝ ∗ v ↦ #ℓ'),
+    <<< ▷ is_infinite_array ap γa ∗ ptr_points_to_segment γa γ v (id `max` id'),
   RET #() >>>.
 Proof.
   iIntros "#HSegLoc HProc" (Φ) "AU". wp_lam. wp_pures. iLöb as "IH".
   wp_bind (!_)%E.
-  iMod "AU" as (id' ℓ') "[[HIsInf [Htl #HLoc]] [HClose _]]".
+  iMod "AU" as (id') "[[HIsInf HPtr] [HClose _]]".
+  iDestruct "HPtr" as (ℓ') "(Htl & #HLoc & HAuth)".
   wp_load.
-  iMod ("HClose" with "[HIsInf Htl HLoc]") as "AU"; first by iFrame.
+  iMod (own_update with "HAuth") as "[HAuth HFrag]".
+  { apply auth_update_core_id with (b := id'); try done. apply _. }
+  iMod ("HClose" with "[HIsInf Htl HLoc HAuth]") as "AU";
+    first by eauto with iFrame.
   iModIntro. wp_pures.
   wp_bind (segment_id #ℓ').
 
   awp_apply segment_id_spec without "HProc".
   iApply (aacc_aupd_abort with "AU"); first done.
-  iIntros (? ?) "[HIsInf HTl]".
+  iIntros (?) "[HIsInf HPtr]".
   iDestruct (is_segment_by_location with "HLoc HIsInf")
     as (? ?) "[HIsSeg HArrRestore]".
   iAaccIntro with "HIsSeg"; iFrame; iIntros "HIsSeg"; iModIntro;
@@ -104,7 +118,7 @@ Proof.
 
   awp_apply segment_id_spec without "HProc".
   iApply (aacc_aupd with "AU"); first done.
-  iIntros (? ?) "[HIsInf HTl]".
+  iIntros (id'') "[HIsInf HPtr]".
   iDestruct (is_segment_by_location with "HSegLoc HIsInf")
     as (? ?) "[HIsSeg HArrRestore]".
   iAaccIntro with "HIsSeg"; iFrame; iIntros "HIsSeg"; iModIntro;
@@ -114,27 +128,44 @@ Proof.
   destruct (decide (id <= id')) eqn:E.
   {
     iRight. iSplitL.
-    { iDestruct "HTl" as "[HTl HLoc']". iRight. iFrame. admit. }
+    { iAssert (⌜id' <= id''⌝)%I with "[HFrag HPtr]" as %HLt.
+      { iDestruct "HPtr" as (?) "(_ & _ & HAuth)".
+        iDestruct (own_valid_2 with "HAuth HFrag")
+          as %[HH%mnat_included _]%auth_both_valid.
+        iPureIntro. lia.
+      }
+      replace (id `max` id'')%nat with id''. done. lia. }
     iIntros "HΦ !> HProc". wp_pures. rewrite bool_decide_decide E. by wp_pures.
   }
   iLeft. iFrame. iIntros "AU !> HProc". wp_pures. rewrite bool_decide_decide E.
   wp_pures.
 
   wp_bind (CmpXchg _ _ _).
-  iMod "AU" as (id'' ℓ'') "[[HIsInf [Htl #HLocs]] HClose]".
+  iMod "AU" as (?) "[[HIsInf HPtr] HClose]".
+  iDestruct "HPtr" as (ℓ'') "(Htl & #HLocs & HAuth)".
 
   destruct (decide (ℓ'' = ℓ')); subst.
   {
     wp_cmpxchg_suc.
-    iMod ("HClose" with "[HIsInf Htl]") as "HΦ".
-    { iFrame. iLeft. iFrame. iPureIntro. admit. }
+    iDestruct (segment_location_id_agree with "HIsInf HLoc HLocs") as %<-.
+    iMod (own_update with "HAuth") as "[HAuth _]".
+    { apply auth_update_alloc. apply (mnat_local_update _ _ id). lia. }
+    iMod ("HClose" with "[HIsInf Htl HAuth]") as "HΦ".
+    { rewrite Max.max_l. iFrame. iExists _. by iFrame. lia. }
     iModIntro. by wp_pures.
   }
   {
     wp_cmpxchg_fail.
     iDestruct "HClose" as "[HClose _]".
-    iMod ("HClose" with "[HIsInf Htl]") as "AU"; first by iFrame.
+    iMod ("HClose" with "[HIsInf Htl HAuth]") as "AU";
+      first by eauto with iFrame.
     iModIntro. wp_pures. wp_lam. wp_pures.
     iApply ("IH" with "HProc AU").
   }
 Qed.
+
+Notation iteratorUR := (prodUR (optionUR positiveR) mnatUR).
+Notation deqIteratorUR := iteratorUR.
+Notation enqIteratorUR := iteratorUR.
+
+End proof.
