formal-proofs/theories/lib/util/interruptibly.v
@@ -33,7 +33,7 @@ Class interruptiblyG Σ := InterruptiblyG {
 }.
 
 Definition interruptiblyΣ : gFunctors :=
-  #[(*GFunctor (exclR unitO);*) GFunctor (authR mnatUR)].
+  #[GFunctor (authR mnatUR)].
 
 Instance subG_interruptiblyΣ {Σ} : subG interruptiblyΣ Σ -> interruptiblyG Σ.
 Proof. solve_inG. Qed.
@@ -42,13 +42,11 @@ Section interruptibly_proof.
 
 Context `{heapG Σ} `{interruptiblyG Σ} (N: namespace).
 
-Definition interrupt_handle_inv γ (H: val) :=
-  (∃ (ℓ: loc), ⌜H = #ℓ⌝ ∧
-               ∃ (n: nat), ℓ ↦ #n ∗ own γ (● (n: mnatUR)) ∧
-                           ⌜n <= 2⌝)%I.
+Definition interrupt_handle_inv γ (ℓ: loc) :=
+  (∃ (n: nat), ℓ ↦ #n ∗ own γ (● (n: mnatUR)) ∧ ⌜n <= 2⌝)%I.
 
 Definition is_interrupt_handle γ H :=
-  inv N (interrupt_handle_inv γ H).
+  (∃ (ℓ: loc), ⌜H = #ℓ⌝ ∧ inv N (interrupt_handle_inv γ ℓ))%I.
 
 Definition interrupted γ := own γ (◯ (2%nat : mnatUR)).
 
@@ -69,41 +67,25 @@ Lemma interruptibly_wait_fail_spec : forall γ handle (b e: val),
     wait handle b e
   {{{ RET (InjLV #()); True }}}.
 Proof.
-  intros.
-  iIntros "[#IntHInv #IntSent] HPost".
-  rewrite /is_interrupt_handle /interrupt_sent /wait.
-  rewrite /interrupt_handle_inv. wp_pures. wp_bind (!_)%E.
-  iInv N as "HInv" "HClose".
-  iDestruct "HInv" as (ℓ) "[>% Hn]".
-  iDestruct "Hn" as (n) "[Hℓ [HOwn >%]]".
-  subst.
+  iIntros (γ handle b e Φ) "[#IntHInv #IntSent] HPost". wp_lam. wp_pures.
+  iDestruct "IntHInv" as (ℓ) "[-> IntHInv]". rewrite /interrupt_handle_inv.
+  wp_bind (!_)%E.
+  iInv N as (n) "(Hℓ & HOwn & >%)" "HClose".
   wp_load.
   destruct n.
-  - iDestruct (own_valid_2 with "HOwn IntSent") as %Hv.
-    apply auth_valid_discrete in Hv; simpl in *.
-    rewrite ucmra_unit_left_id in Hv.
-    destruct Hv as [_ [a [Contra1 [Contra2 _]]]].
-    apply to_agree_inj in Contra1.
-    inversion Contra1; subst.
-    apply mnat_included in Contra2.
-    inversion Contra2.
-  - iMod ("HClose" with "[Hℓ HOwn]") as "_"; first by eauto 10 with iFrame.
-    iModIntro.
-    wp_pures.
-    wp_bind (_ <- _)%E.
-    iInv N as "HInv" "HClose".
-    iDestruct "HInv" as (ℓ') "[>% Hn]".
-    iDestruct "Hn" as (n') "[Hℓ [HOwn >%]]".
-    inversion H1; subst.
-    wp_store.
-    iMod (own_update with "HOwn") as "[HOwn HFrag]".
-    {
-      apply (auth_update_alloc _ (2%nat: mnatUR) (2%nat: mnatUR)).
-      apply mnat_local_update.
-      lia.
-    }
-    iMod ("HClose" with "[Hℓ HOwn]") as "_"; first by eauto 10 with iFrame.
-    iModIntro. wp_pures. by iApply "HPost".
+  by iDestruct (own_valid_2 with "HOwn IntSent")
+      as %[HC%mnat_included _]%auth_both_valid; lia.
+
+  iMod ("HClose" with "[Hℓ HOwn]") as "_"; first by eauto 10 with iFrame.
+  iModIntro. wp_pures. wp_bind (_ <- _)%E.
+
+  iInv N as (?) "(Hℓ & HOwn & >%)" "HClose".
+  wp_store.
+  iMod (own_update with "HOwn") as "[HOwn HFrag]".
+  { apply (auth_update_alloc _ (2%nat: mnatUR) (2%nat: mnatUR)).
+    apply mnat_local_update. lia. }
+  iMod ("HClose" with "[Hℓ HOwn]") as "_"; first by eauto 10 with iFrame.
+  iModIntro. wp_pures. by iApply "HPost".
 Qed.
 
 Lemma interruptibly_wait_spec : forall γ P Q handle (b e: val),
@@ -116,47 +98,25 @@ Lemma interruptibly_wait_spec : forall γ P Q handle (b e: val),
   {{{ r, RET r; ⌜r = InjLV #()⌝ ∧ P ∧ interrupted γ ∨
                                         (∃ (v: val), ⌜r = InjRV v⌝ ∧ Q v )}}}.
 Proof.
-  intros.
-  iIntros "[#IntHInv [HP #Hbe]]"; rewrite /is_interrupt_handle.
-  iIntros "HPost".
-  iLöb as "IH". wp_lam. wp_pures.
-  wp_bind (!_)%E.
-  iInv N as "HInv" "HClose".
-  rewrite /interrupt_handle_inv.
-  iDestruct "HInv" as (ℓ) "[>% Hn]"; subst.
-  iDestruct "Hn" as (n) "[Hℓ [HOwn >%]]".
+  iIntros (γ P Q handle b e Φ) "[#IntHInv [HP #Hbe]] HPost". wp_lam. wp_pures.
+  iDestruct "IntHInv" as (ℓ) "[-> IntHInv]". rewrite /interrupt_handle_inv.
+  iLöb as "IH". wp_bind (!_)%E.
+  iInv N as (n) "[Hℓ [HOwn >%]]" "HClose".
   wp_load.
   destruct n.
   all: iMod ("HClose" with "[Hℓ HOwn]") as "_"; first by eauto 10 with iFrame.
   all: iModIntro; wp_pures.
-  - wp_bind (b e).
-    wp_apply ("Hbe" with "HP").
-    iIntros (r) "H".
-    iDestruct "H" as "[[% HP]|HR]"; subst.
-    * wp_pures.
-      by wp_apply ("IH" with "HP").
-    * iDestruct "HR" as (v) "[% HQ]"; subst.
-      wp_pures.
-      iApply "HPost".
-      eauto.
+  - wp_bind (b e). wp_apply ("Hbe" with "HP"). iIntros (r) "[[-> HP]|HR]".
+    * wp_pures. wp_lam. wp_pures. by wp_apply ("IH" with "HP").
+    * iDestruct "HR" as (v) "[-> HQ]". wp_pures. iApply "HPost". eauto.
   - wp_bind (_ <- _)%E.
-    iInv N as "HInv" "HClose".
-    iDestruct "HInv" as (ℓ') "[>% Hn]"; subst.
-    inversion H2; subst.
-    iDestruct "Hn" as (n') "[Hℓ [HOwn >%]]".
+    iInv N as (n') "[Hℓ [HOwn >%]]" "HClose".
     wp_store.
     iMod (own_update with "HOwn") as "[HOwn HFrag]".
-    {
-      apply (auth_update_alloc _ (2%nat: mnatUR) (2%nat: mnatUR)).
-      apply mnat_local_update.
-      lia.
-    }
+    { apply (auth_update_alloc _ (2%nat: mnatUR) (2%nat: mnatUR)).
+      apply mnat_local_update. lia. }
     iMod ("HClose" with "[Hℓ HOwn]") as "_"; first by eauto 10 with iFrame.
-    iModIntro.
-    wp_pures.
-    iApply "HPost".
-    iLeft.
-    rewrite /interrupted.
+    iModIntro. wp_pures. iApply "HPost". iLeft. rewrite /interrupted.
     eauto with iFrame.
 Qed.
 
@@ -169,18 +129,10 @@ Lemma interruptibly_fail_spec : forall γ P Q' handle (b h e: val),
     interruptibly handle b h e
   {{{ (v: val), RET (#true, v)%V; Q' v }}}.
 Proof.
-  intros.
-  iIntros "[#HIsInt [HP [#HIntSent #Hhe]]] HPost".
-  wp_rec.
-  wp_pures.
+  intros. iIntros "[#HIsInt [HP [#HIntSent #Hhe]]] HPost". wp_rec. wp_pures.
   wp_apply (interruptibly_wait_fail_spec); auto.
-  iIntros "_".
-  wp_pures.
-  wp_bind (h e).
-  wp_apply ("Hhe" with "HP").
-  iIntros (r) "HQ'".
-  wp_pures.
-  by iApply "HPost".
+  iIntros "_". wp_pures. wp_bind (h e). wp_apply ("Hhe" with "HP").
+  iIntros (r) "HQ'". wp_pures. by iApply "HPost".
 Qed.
 
 Lemma interruptibly_spec : forall γ P Q Q' handle (b h e: val),
@@ -195,30 +147,13 @@ Lemma interruptibly_spec : forall γ P Q Q' handle (b h e: val),
     interruptibly handle b h e
   {{{ r v, RET r; ⌜r = (#true, v)%V⌝ ∧ Q' v ∨ ⌜r = (#false, InjRV v)%V⌝ ∧ Q v }}}.
 Proof.
-  intros.
-  iIntros "[#HIsInt [HP [#Hbe #Hhe]]] HPost".
-  wp_rec.
-  wp_pures.
-  wp_bind (wait _ _ _).
-  wp_apply (interruptibly_wait_spec with "[HP]").
-  { iSplitR; eauto.
-    iSplitL. iApply "HP".
-    iApply "Hbe". }
-  iIntros (r) "HP".
-  iDestruct "HP" as "[[% [HP HIntr]] | Hr]".
-  - subst. wp_pures.
-    wp_bind (h e).
-    wp_apply ("Hhe" with "[HP HIntr]"); first by iFrame.
-    iIntros (r) "HQ'".
-    wp_pures.
-    iApply "HPost".
-    iLeft.
-    by iFrame.
-  - iDestruct "Hr" as (v) "[% HQ]".
-    subst. wp_pures.
-    iApply "HPost".
-    iRight.
-    by iFrame.
+  intros. iIntros "[#HIsInt [HP [#Hbe #Hhe]]] HPost". wp_rec. wp_pures.
+  wp_bind (wait _ _ _). wp_apply (interruptibly_wait_spec with "[HP]").
+  { iFrame "HIsInt". iSplitL. iApply "HP". iApply "Hbe". }
+  iIntros (r) "[[-> [HP HIntr]] | Hr]".
+  - wp_pures. wp_bind (h e). wp_apply ("Hhe" with "[HP HIntr]"); first by iFrame.
+    iIntros (r) "HQ'". wp_pures. iApply "HPost". iLeft. by iFrame.
+  - iDestruct "Hr" as (v) "[-> HQ]". wp_pures. iApply "HPost". iRight. by iFrame.
 Qed.
 
 Lemma new_handle_spec:
@@ -226,20 +161,14 @@ Lemma new_handle_spec:
     new_handle #()
   {{{ γ H, RET H; is_interrupt_handle γ H }}}.
 Proof.
-  iIntros (Φ) "_ HPost". rewrite /new_handle -wp_fupd.
-  wp_lam. rewrite /is_interrupt_handle.
-  iMod (own_alloc (● (O : mnatUR))) as (γ) "HOwn".
-  { apply auth_valid_discrete. simpl.
-    split. done.
-    by eexists.
-  }
+  iIntros (Φ) "_ HPost". wp_lam.
+  iMod (own_alloc (● (O: mnatUR))) as (γ) "HOwn";
+    first by apply auth_auth_valid.
+  rewrite -wp_fupd.
   wp_alloc ℓ as "Hℓ".
-  iMod (inv_alloc N _ (interrupt_handle_inv γ #ℓ) with "[HOwn Hℓ]") as "HInv".
-  {
-    iNext. rewrite /interrupt_handle_inv. by eauto with iFrame.
-  }
-  iModIntro.
-  by iApply "HPost".
+  iMod (inv_alloc N _ (interrupt_handle_inv γ ℓ) with "[HOwn Hℓ]") as "HInv".
+  { iExists _; by eauto with iFrame. }
+  iModIntro. iApply "HPost". iExists _. eauto.
 Qed.
 
 Lemma interrupt_spec γ handle:
@@ -248,43 +177,21 @@ Lemma interrupt_spec γ handle:
   {{{ v, RET v; interrupt_sent γ }}}.
 Proof.
   iIntros (Φ) "#HIsInt HPost".
-  rewrite /is_interrupt_handle /interrupt.
+  iDestruct "HIsInt" as (ℓ) "[-> IntHInv]". rewrite /interrupt_handle_inv.
   wp_lam. wp_bind (CmpXchg _ _ _).
-  iInv N as "HInv" "HClose".
-  iDestruct "HInv" as (ℓ) "[>% Hn]". subst.
-  iDestruct "Hn" as (n) "[Hℓ [HOwn >%]]".
+  iInv N as (n) "[Hℓ [HOwn >%]]" "HClose".
   destruct n.
   - wp_cmpxchg_suc.
     iMod (own_update with "HOwn") as "[HOwn HFrag]".
-    {
-      apply (auth_update_alloc _ (1%nat: mnatUR) (1%nat: mnatUR)).
-      apply mnat_local_update.
-      lia.
-    }
-    iMod ("HClose" with "[Hℓ HOwn]") as "_".
-    {
-      iNext; iExists ℓ; iSplitR; auto.
-      iExists (S O); iFrame. auto.
-    }
-    iModIntro.
-    wp_pures.
-    iApply "HPost".
-    by rewrite /interrupt_sent.
+    { apply (auth_update_alloc _ (1%nat: mnatUR) (1%nat: mnatUR)).
+      apply mnat_local_update. lia. }
+    iMod ("HClose" with "[Hℓ HOwn]") as "_". by eauto with iFrame.
+    iModIntro. wp_pures. iApply "HPost". by rewrite /interrupt_sent.
   - wp_cmpxchg_fail; first done.
     iMod (own_update with "HOwn") as "[HOwn HFrag]".
-    {
-      apply (auth_update_core_id _ (1%nat: mnatUR)).
-      apply mnat_included.
-      lia.
-    }
-    iMod ("HClose" with "[Hℓ HOwn]") as "_".
-    {
-      iExists _. eauto 10 with iFrame.
-    }
-    iModIntro.
-    wp_pures.
-    iApply "HPost".
-    by rewrite /interrupt_sent.
+    { apply (auth_update_core_id _ (1%nat: mnatUR)). apply mnat_included. lia. }
+    iMod ("HClose" with "[Hℓ HOwn]") as "_". by eauto with iFrame.
+    iModIntro. wp_pures. iApply "HPost". by rewrite /interrupt_sent.
  Qed.
 
 End interruptibly_proof.
